assume populate memory and implement kf for 2d blocktiling

src/lib/poly/gemm/Kuiper.Poly.GEMM.BlockTiling2D.fst
@@ -72,11 +72,11 @@ let kpre1
   (eB : ematrix4 et mshared mcols bk bn)
   (fA fB : perm)
   (bid : natlt (mrows * mcols))
-  (tid : natlt (bm/tm * bn/tn))
+  (tid : natlt (bm/tm * (bn/tn)))
   : slprop
   =
-  (gA |-> Frac (fA /. (mrows * mcols * (bm/tm * bn/tn))) eA) **
-  (gB |-> Frac (fB /. (mrows * mcols * (bm/tm * bn/tn))) eB) **
+  (gA |-> Frac (fA /. (mrows * mcols * (bm/tm * (bn/tn)))) eA) **
+  (gB |-> Frac (fB /. (mrows * mcols * (bm/tm * (bn/tn)))) eB) **
   (forall+ (i : natlt tm) (j : natlt tn).
     (exists* v.
       m4_pts_to_cell gC
@@ -104,11 +104,11 @@ let kpost1
   (eB : ematrix4 et mshared mcols bk bn)
   (fA fB : perm)
   (bid : natlt (mrows * mcols))
-  (tid : natlt (bm/tm * bn/tn))
+  (tid : natlt (bm/tm * (bn/tn)))
   : slprop
   =
-  (gA |-> Frac (fA /. (mrows * mcols * (bm/tm * bn/tn))) eA) **
-  (gB |-> Frac (fB /. (mrows * mcols * (bm/tm * bn/tn))) eB) **
+  (gA |-> Frac (fA /. (mrows * mcols * (bm/tm * (bn/tn)))) eA) **
+  (gB |-> Frac (fB /. (mrows * mcols * (bm/tm * (bn/tn)))) eB) **
   (forall+ (i : natlt tm) (j : natlt tn).
     (exists* v.
       m4_pts_to_cell gC
@@ -138,8 +138,8 @@ let own_tile_stride_cells
   (tid : natlt nthr)
   : slprop
   =
-  forall+ (iter : natlt (div_ceil (rows*cols) nthr)).
-    let flat_idx = iter * nthr + tid <: nat in
+  forall+ (it : natlt (div_ceil (rows*cols) nthr)).
+    let flat_idx = tid + (it * nthr) <: nat in
     let i = flat_idx/cols <: nat in
     let j = flat_idx%cols <: nat in
       // if (flat_idx < rows*cols)
@@ -152,7 +152,7 @@ fn cp_tile
   (#et : Type0) {| scalar et |}
   (#brows #bcols #mrows #mcols: szp)
   (#slM : mlayout brows bcols) {| clayout slM |}
-  // this should just be a submatrix dst
+  // this should just be a submatrix dst 
   (sM : gpu_matrix et slM)
   (#esM : ematrix et brows bcols)
   (#lA : mlayout4 mrows mcols brows bcols)
@@ -174,20 +174,25 @@ fn cp_tile
   unfold own_tile_stride_cells sM esM nthr tid;
   let mlen = mrows *^ brows *^ mcols *^ bcols;
   admit();
-  let mut i = tid;
+
+  let mut i: sz = tid;
   while (SZ.(!i <^ mlen))
-    invariant
-      exists* (ite: sz) (vflatIdx: sz{vflatIdx < mlen}).
-        (pure(ite * nthr + tid == vflatIdx)) **
-        (i |-> vflatIdx) //**
-        // (gpu_matrix_pts_to_cell sM
-        //   ((ite*nthr+tid)/bcols) ((ite*nthr+tid%bcols))
-        //   (macc eM ((ite*nthr+tid)/bcols) ((ite*nthr+tid%bcols))))// **
+    invariant b.
+      (if (b = true) then 
+        exists* (vi : sz{vi < mlen}) (ite: sz).
+          (pure(b == vi < mlen)) **
+          (pure(tid + (ite * nthr) == vi)) **
+          (i |-> vi)
+          // (gpu_matrix_pts_to_cell sM
+          //   (vi/bcols) (vi%bcols) 
+          //   (macc eM (vi/bcols) (vi)))// **
+       else emp) //**
         // (forall+ (ii: natlt ite).
         //   gpu_matrix_pts_to_cell gM
         //     ((ii*nthr+tid)/bcols) ((ii*nthr+tid)%bcols)
         //     (macc eM ((ii*nthr+tid)/bcols) ((ii*nthr+tid)%bcols)))
   {
+    admit();
     let v = M4.gpu_matrix_read gM mrow mcol (!i /^ bcols) (!i %^ bcols);
     M.gpu_matrix_write_cell sM (!i /^ bcols) (!i %^ bcols) v;
 
@@ -200,8 +205,8 @@ fn cp_tile
 let barrier_p
   (#et : Type0)
   (#bm #bn #bk : szp)
-  (#l1 : mlayout bm bk)
-  (#l2 : mlayout bk bn)
+  (#l1 : mlayout bm bk) 
+  (#l2 : mlayout bk bn) 
   (m1 : gpu_matrix et l1)
   (m2 : gpu_matrix et l2)
   (nthr : pos)
@@ -217,7 +222,7 @@ let barrier_p
 let barrier_q
   (#et : Type0)
   (#bm #bn #bk : szp)
-  (#l1 : mlayout bm bk)
+  (#l1 : mlayout bm bk) 
   (#l2 : mlayout bk bn)
   (m1 : gpu_matrix et l1)
   (m2 : gpu_matrix et l2)
@@ -248,7 +253,7 @@ unfold
 let kpre
   (#et : Type0) {| scalar et |}
   (comb : binop et)
-  (#bm #bn #bk : szp)
+  (#bm #bn #bk : szp{SZ.fits (bm * bk) /\ SZ.fits (bk * bn)})
   (#mrows #mshared #mcols : szp)
   (tm : szp{tm /? bm})
   (tn : szp{tn /? bn})
@@ -265,20 +270,19 @@ let kpre
   (fA fB : perm)
   (sh : c_shmems (shmems_desc et bm bn bk))
   (bid : natlt (mrows * mcols))
-  (tid : natlt (bm/tm * bn/tn))
+  (tid : natlt (bm/tm * (bn/tn)))
   : slprop
   =
   kpre1 comb tm tn gA gB gC eA eB fA fB bid tid **
-  (exists* (x : seq _). fst sh |-> Frac (1.0R /. (bm/tm * bn/tn)) x) **
-  (exists* (x : seq _). fst (snd sh) |-> Frac (1.0R /. (bm/tm * bn/tn)) x) **
-  barrier_tok slA slB (fst sh) (fst (snd sh)) 0 (bm/tm * bn/tn) tid
+  (exists* (x : seq _). fst sh |-> Frac (1.0R /. (bm/tm * (bn/tn))) x) **
+  (exists* (x : seq _). fst (snd sh) |-> Frac (1.0R /. (bm/tm * (bn/tn))) x) **
+  barrier_tok slA slB (fst sh) (fst (snd sh)) 0 (bm/tm * (bn/tn)) tid
 
 unfold
 let kpost
   (#et : Type0) {| scalar et |}
   (comb : binop et)
-  (#bm #bn #bk : szp)
-  (#_ : squash (SZ.fits (bm * bk) /\ SZ.fits (bk * bn)))
+  (#bm #bn #bk : szp{SZ.fits (bm * bk) /\ SZ.fits (bk * bn)})
   (#mrows #mshared #mcols : szp)
   (tm : szp{tm /? bm})
   (tn : szp{tn /? bn})
@@ -295,14 +299,42 @@ let kpost
   (fA fB : perm)
   (sh : c_shmems (shmems_desc et bm bn bk))
   (bid : natlt (mrows * mcols))
-  (tid : natlt (bm/tm * bn/tn))
+  (tid : natlt (bm/tm * (bn/tn)))
   : slprop
   =
-  kpre comb tm tn slA slB gA gB gC eA eB fA fB sh bid tid
-  // kpost1 comb tm tn gA gB gC eA eB fA fB bid tid **
-  // (exists* (x : seq _). fst sh |-> Frac (1.0R /. (bm/tm * bn/tn)) x) **
-  // (exists* (x : seq _). fst (snd sh) |-> Frac (1.0R /. (bm/tm * bn/tn)) x) **
-  // barrier_tok slA slB (fst sh) (fst (snd sh)) 0 (bm/tm * bn/tn) tid
+  kpost1 comb tm tn gA gB gC eA eB fA fB bid tid **
+  (exists* (x : seq _). fst sh |-> Frac (1.0R /. (bm/tm * bn/tn)) x) **
+  (exists* (x : seq _). fst (snd sh) |-> Frac (1.0R /. (bm/tm * bn/tn)) x) **
+  barrier_tok slA slB (fst sh) (fst (snd sh)) (2 * mshared) (bm/tm * bn/tn) tid
+
+let own_cell_in_each_tile
+  (#et : Type0)
+  (#mrows #brows #bcols: nat)
+  (#lm : mlayout4 mrows 1 brows bcols)
+  (m : gpu_matrix4 et lm)
+  (em : ematrix4 et mrows 1 brows bcols)
+  (tid : natlt (brows*bcols))
+  : slprop
+  =
+  forall+ (i: natlt mrows).
+    M4.gpu_matrix_pts_to_cell m i 0 (tid/bcols) (tid%bcols) (macc em i 0 (tid/bcols) (tid%bcols))
+
+// #push-options "--retry 6"
+// let constraint_test
+//   (#bm #bn #bk : szp)
+//   (tm : szp{tm /? bm})
+//   (tn : szp{tn /? bn})
+
+//   (#_ : squash (bm/tm*(bn/tn)/bk /? bm /\ bk /? (bm/tm*(bn/tn)) /\
+//                 bm/tm*(bn/tn)/bn /? bk /\ bn /? (bm/tm*(bn/tn))))
+//   =
+//   assert (bm == bn);
+//   assert ((bm/tm * (bn/tn)) == bm*bn/(tm*tn));
+//   // assert ((bm/tm * bm) == bm * bk /\ (bm/tm * bm) == bn * bk);
+//   // assert ((bm/tm * bm) == bm * bk /\ bm * bk == bn * bk);
+//   // assert ((bm/tm * bm) == bm * bk /\ bm == bn);
+//   // assert (SZ.v bm == tm * bk /\ bm == bn);
+//   ()
 
 inline_for_extraction noextract
 fn populate_shmem
@@ -311,6 +343,9 @@ fn populate_shmem
   (#mrows #mshared #mcols : erased nat)
   (tm : szp{tm /? bm})
   (tn : szp{tn /? bn})
+  // restriction required by the original code
+  // (#_ : squash (bm/tm*(bn/tn)/bk /? bm /\ bk /? (bm/tm*(bn/tn)) /\
+  //               bm/tm*(bn/tn)/bn /? bk /\ bn /? (bm/tm*(bn/tn))))
   (#slA : mlayout bm bk) {| clayout slA |}
   (#slB : mlayout bk bn) {| clayout slB |}
   (sA : gpu_matrix et slA)
@@ -327,13 +362,15 @@ fn populate_shmem
   (mrow : szlt mrows)
   (mk : szlt mshared)
   (mcol : szlt mcols)
-  (tid : szlt (bm/tm * bn/tn))
+  (tid : szlt (bm/tm * (bn/tn)))
   preserves
     gpu **
     (gA |-> Frac fA eA) **
+    (gB |-> Frac fB eB) **
     (exists* (eA: _) (eB: _).
-      own_tile_stride_cells sA eA (bm/tm * bn/tn) **
-      own_tile_stride_cells sB eB (bm/tm * bn/tn))
+      // own_in_each_tile sA eA bm bn tid)
+      own_tile_stride_cells sA eA (bm/tm * (bn/tn)) tid **
+      own_tile_stride_cells sB eB (bm/tm * (bn/tn)) tid)
 {
   admit();
   // unfold own_1_cell sA (tid/bk) (tid%bk);
@@ -388,12 +425,12 @@ fn subproducts2d
   let mut dotIdx : sz = 0sz;
   while (SZ.(!dotIdx <^ bk))
     invariant
-      exists* (vdotIdx : sz{vdotIdx <= bk}) (vrAcol0 : erased (lseq et tm))
-        (vrBrow0 : erased (lseq et tn)) (vrchProd0 : erased (lseq et (tm*tn))).
+      exists* (vdotIdx : sz{vdotIdx <= bk}) (vrAcol : erased (lseq et tm))
+        (vrBrow : erased (lseq et tn)) (vrchProd : erased (lseq et (tm*tn))).
         (dotIdx |-> vdotIdx) **
-        (rAcol |-> vrAcol0) **
-        (rBrow |-> vrBrow0) **
-        (rchProd |-> vrchProd0)
+        (rAcol |-> vrAcol) **
+        (rBrow |-> vrBrow) **
+        (rchProd |-> vrchProd)
   {
     open Pulse.Lib.Array;
 
@@ -465,16 +502,16 @@ fn subproducts2d
 
 // even 20 isn't evenough for the checking from the terminal
 //  (but enough for the vs code extension)
-#push-options "--z3rlimit 30"
+#push-options "--z3rlimit 30 --retry 6"
+#push-options "--debug SMTFail --split_queries always"
 inline_for_extraction noextract
 fn kf
   (#et : Type0) {| scalar et |}
   (comb : binop et)
-  (#bm #bn #bk : szp)
+  (#bm #bn #bk : szp{SZ.fits (bm * bk) /\ SZ.fits (bk * bn)})
   (#mrows #mshared #mcols : szp)
   (tm : szp{tm /? bm})
-  (#_: squash ((bm/tm * bn) == bm * bk /\ (bm/tm * bn) == bn * bk))
-  (#_ : squash (SZ.fits (bm * bk) /\ SZ.fits (bk * bn)))
+  (tn : szp{tn /? bn})
   (slA : mlayout bm bk)
   (slB : mlayout bk bn)
   {| clayout slA, clayout slB |}
@@ -487,21 +524,21 @@ fn kf
   (gB : gpu_matrix4 et lB)
   (#fB : perm)
   (gC : gpu_matrix4 et lC)
-  (#eA : ematrix4 et mrows   mshared bm bk)
-  (#eB : ematrix4 et mshared mcols   bk bn)
+  (#eA : ematrix4 et mrows mshared bm bk)
+  (#eB : ematrix4 et mshared mcols bk bn)
   (sh : c_shmems (shmems_desc et bm bn bk))
   (bid : szlt (mrows * mcols))
-  (tid : szlt (bm/tm * bn))
+  (tid : szlt (bm/tm * (bn/tn)))
   ()
   requires
     gpu **
-    kpre comb tm slA slB gA gB gC eA eB fA fB sh bid tid **
-    thread_id (bm/tm * bn) tid **
+    kpre comb tm tn slA slB gA gB gC eA eB fA fB sh bid tid **
+    thread_id (bm/tm * (bn/tn)) tid **
     block_id (mrows * mcols) bid
   ensures
     gpu **
-    kpost comb tm slA slB gA gB gC eA eB fA fB sh bid tid **
-    thread_id (bm/tm * bn) tid **
+    kpost comb tm tn slA slB gA gB gC eA eB fA fB sh bid tid **
+    thread_id (bm/tm * (bn/tn)) tid **
     block_id (mrows * mcols) bid
 {
   let sarA : gpu_array et (bm * bk) = fst sh;
@@ -512,7 +549,7 @@ fn kf
   gpu_pts_to_ref sarA;
   gpu_pts_to_ref sarB;
 
-  unfold barrier_tok tm slA slB sarA sarB 0 tid;
+  unfold barrier_tok slA slB sarA sarB 0 (bm/tm * (bn/tn)) tid;
 
   M.gpu_matrix_abs' slA sarA;
   let sA = M.from_array slA sarA;
@@ -525,186 +562,199 @@ fn kf
 
   let mrow = bid /^ mcols;
   let mcol = bid %^ mcols;
-  let threadRow = tid /^ bn;
-  let threadCol = tid %^ bn;
+  let threadRow = tid /^ (bn/^tn);
+  let threadCol = tid %^ (bn/^tn);
 
-  (* thread-local result cache *)
-  let mut cache1d : Pulse.Lib.Array.array et = [| zero #et #_ ; tm |];
+  (* register caches *)
+  let mut rAcol : Pulse.Lib.Array.array et = [| zero #et #_ ; tm |];
+  let mut rBrow : Pulse.Lib.Array.array et = [| zero #et #_ ; tn |];
+  let mut rchProd : Pulse.Lib.Array.array et = [| zero #et #_ ; tm*^tn |];
 
   let mut bkIdx  : sz = 0sz;
   while (SZ.(!bkIdx <^ mshared))
     invariant b.
-      exists* (vbkIdx : SZ.t{vbkIdx <= mshared}) (cache1dv : lseq et tm).
+      exists* (vbkIdx : SZ.t{vbkIdx <= mshared}) (vrAcol : lseq et tm) (vrBrow : lseq et tn) (vrchProd : lseq et (tm*tn)).
         pure (b == (SZ.v vbkIdx < mshared)) **
         (bkIdx |-> vbkIdx) **
-        (cache1d |-> cache1dv) **
-        (gA |-> Frac (fA /. (mrows * mcols * (bm/tm * bn))) eA) **
-        (gB |-> Frac (fB /. (mrows * mcols * (bm/tm * bn))) eB) **
-        (exists* (x : ematrix _ _ _). sA |-> Frac (1.0R /. (bm/tm * bn)) x) **
-        (exists* (x : ematrix _ _ _). sB |-> Frac (1.0R /. (bm/tm * bn)) x) **
-        B.barrier_tok (barrier_p tm sA sB) (barrier_q tm sA sB) (2 * vbkIdx) tid **
+        (rAcol |-> vrAcol) **
+        (rBrow |-> vrBrow) **
+        (rchProd |-> vrchProd) **
+        (gA |-> Frac (fA /. (mrows * mcols * (bm/tm * (bn/tn)))) eA) **
+        (gB |-> Frac (fB /. (mrows * mcols * (bm/tm * (bn/tn)))) eB) **
+        (exists* (x : ematrix _ _ _). sA |-> Frac (1.0R /. (bm/tm * (bn/tn))) x) **
+        (exists* (x : ematrix _ _ _). sB |-> Frac (1.0R /. (bm/tm * (bn/tn))) x) **
+        B.barrier_tok (barrier_p sA sB (bm/tm * (bn/tn))) (barrier_q sA sB (bm/tm * (bn/tn))) (2 * vbkIdx) tid **
         gpu
   {
     (* This assert should not be needed. I don't know what effect it even has. *)
     let vbkIdx = !bkIdx;
-    assert B.barrier_tok (barrier_p tm sA sB) (barrier_q tm sA sB) (2 * vbkIdx) tid;
+    assert B.barrier_tok (barrier_p sA sB (bm/tm * (bn/tn))) (barrier_q sA sB (bm/tm * (bn/tn))) (2 * vbkIdx) tid;
     even_2x vbkIdx;
     rewrite
-        (exists* (x : ematrix _ _ _). sA |-> Frac (1.0R /. (bm/tm * bn)) x) **
-        (exists* (x : ematrix _ _ _). sB |-> Frac (1.0R /. (bm/tm * bn)) x)
-      as barrier_p tm sA sB (2 * vbkIdx) tid;
+        (exists* (x : ematrix _ _ _). sA |-> Frac (1.0R /. (bm/tm * (bn/tn))) x) **
+        (exists* (x : ematrix _ _ _). sB |-> Frac (1.0R /. (bm/tm * (bn/tn))) x)
+      as barrier_p sA sB (bm/tm * (bn/tn)) (2 * vbkIdx) tid;
 
     B.barrier_wait ();
-    rewrite (barrier_q tm sA sB (2 * vbkIdx) tid)
-         as own_1_cell sA (tid /^ bk) (tid%bk) ** own_1_cell sB (tid/bn) (tid%bn);
+    rewrite (barrier_q sA sB (bm/tm * (bn/tn)) (2 * vbkIdx) tid)
+        as (exists* (em: ematrix _ _ _). own_tile_stride_cells sA em (bm/tm * (bn/tn)) tid) **
+           (exists* (em: ematrix _ _ _). own_tile_stride_cells sB em (bm/tm * (bn/tn)) tid);
 
-    (* At this point we exclusively own a full column of the SHMEM
-       cache. Populate it. *)
-    populate_shmem tm sA sB gA gB mrow !bkIdx mcol tid;
+    populate_shmem tm tn sA sB gA gB mrow !bkIdx mcol tid;
 
-    assert (B.barrier_tok (barrier_p tm sA sB) (barrier_q tm sA sB) (2 * vbkIdx + 1) tid);
+    assert (B.barrier_tok (barrier_p sA sB (bm/tm * (bn/tn))) (barrier_q sA sB (bm/tm * (bn/tn))) (2 * vbkIdx + 1) tid);
     odd_2x1 vbkIdx;
     assert (pure (odd (2 * vbkIdx + 1)));
-    rewrite own_1_cell sA (tid/bk) (tid%bk) ** own_1_cell sB (tid/bn) (tid%bn)
-         as (barrier_p tm sA sB (2 * vbkIdx + 1) tid);
+    rewrite (exists* (em: ematrix _ _ _). own_tile_stride_cells sA em (bm/tm * (bn/tn)) tid) **
+           (exists* (em: ematrix _ _ _). own_tile_stride_cells sB em (bm/tm * (bn/tn)) tid)
+         as (barrier_p sA sB (bm/tm * (bn/tn)) (2 * vbkIdx + 1) tid);
+
     B.barrier_wait ();
+
     even_2x (vbkIdx + 1);
-    (* sigh *)
     assert (pure (2 * (vbkIdx + 1) == 2 * vbkIdx + 2));
     assert (pure (even (2 * vbkIdx + 2)));
-    rewrite (barrier_q tm sA sB (2 * vbkIdx + 1) tid)
+    rewrite (barrier_q sA sB (bm/tm * (bn/tn)) (2 * vbkIdx + 1) tid)
     as
-      (exists* (x : ematrix _ _ _). sA |-> Frac (1.0R /. (bm/tm * bn)) x) **
-      (exists* (x : ematrix _ _ _). sB |-> Frac (1.0R /. (bm/tm * bn)) x);
+      (exists* (x : ematrix _ _ _). sA |-> Frac (1.0R /. (bm/tm * (bn/tn))) x) **
+      (exists* (x : ematrix _ _ _). sB |-> Frac (1.0R /. (bm/tm * (bn/tn))) x);
 
-    subproducts1d tm cache1d sA sB threadRow threadCol;
+    subproducts2d tm tn rAcol rBrow rchProd sA sB threadRow threadCol;
 
-    (* Move to next tile *)
     bkIdx := !bkIdx +^ 1sz;
   };
 
+  forevery_flatten #(natlt tm) #_ #(natlt tn) _;
   ghost
-  fn aux (i: natlt tm)
+  fn aux (i: (natlt tm & natlt tn))
   requires
     (exists* (v: et).
       M4.gpu_matrix_pts_to_cell #et #(SZ.v mrows) #(SZ.v mcols) #(SZ.v bm)
         #(SZ.v bn) #lC gC #1.0R (SZ.v bid / SZ.v mcols)
-        (SZ.v bid % SZ.v mcols) (SZ.v tid / SZ.v bn * SZ.v tm + i)
-        (SZ.v tid % SZ.v bn) v)
+        (SZ.v bid % SZ.v mcols) (SZ.v tid / (SZ.v bn / SZ.v tn) * SZ.v tm + i._1)
+        (SZ.v tid % (SZ.v bn / SZ.v tn) * SZ.v tn + i._2) v)
   ensures
     (exists* (v: et).
       M4.gpu_matrix_pts_to_cell #et #(SZ.v mrows) #(SZ.v mcols) #(SZ.v bm)
         #(SZ.v bn) #lC gC #1.0R (SZ.v mrow)
-        (SZ.v mcol) (SZ.v threadRow * SZ.v tm + i)
-        (SZ.v threadCol) v)
+        (SZ.v mcol) (SZ.v threadRow * SZ.v tm + i._1)
+        (SZ.v threadCol * SZ.v tn + i._2) v)
   {
     with v. _;
     rewrite
       (M4.gpu_matrix_pts_to_cell #et #(SZ.v mrows) #(SZ.v mcols) #(SZ.v bm)
-          #(SZ.v bn) #lC gC #1.0R (SZ.v bid / SZ.v mcols)
-          (SZ.v bid % SZ.v mcols) (SZ.v tid / SZ.v bn * SZ.v tm + i)
-          (SZ.v tid % SZ.v bn) v)
-    as
+        #(SZ.v bn) #lC gC #1.0R (SZ.v bid / SZ.v mcols)
+        (SZ.v bid % SZ.v mcols) (SZ.v tid / (SZ.v bn / SZ.v tn) * SZ.v tm + i._1)
+        (SZ.v tid % (SZ.v bn / SZ.v tn) * SZ.v tn + i._2) v)
+    as 
       (M4.gpu_matrix_pts_to_cell #et #(SZ.v mrows) #(SZ.v mcols) #(SZ.v bm)
-          #(SZ.v bn) #lC gC #1.0R (SZ.v (bid /^ mcols))
-          (SZ.v (bid %^ mcols)) (SZ.v (tid /^ bn) * SZ.v tm + i)
-          (SZ.v (tid %^ bn)) v);
-    rewrite each SZ.v (bid /^ mcols) as SZ.v mrow,
-                 SZ.v (bid %^ mcols) as SZ.v mcol,
-                 SZ.v (tid /^ bn) as SZ.v threadRow,
-                 SZ.v (tid %^ bn) as SZ.v threadCol;
+        #(SZ.v bn) #lC gC #1.0R (SZ.v mrow)
+        (SZ.v mcol) (SZ.v threadRow * SZ.v tm + i._1)
+        (SZ.v threadCol * SZ.v tn + i._2) v);
     ()
   };
   forevery_map _ _ aux;
 
   (* Write all the accumulated dotproducts. *)
-  let mut resIdx : sz = 0sz;
-  Pulse.Lib.Array.pts_to_len cache1d;
-  while (SZ.(!resIdx <^ tm))
-    invariant b.
-      exists* (vresIdx : SZ.t{vresIdx <= tm}) (dotpv : lseq et tm).
-        pure (b == (SZ.v vresIdx < tm)) **
-        (resIdx |-> vresIdx) **
-        (cache1d |-> dotpv) **
-        (forall+ (ii : natlt tm).
-          (exists* v.
-            m4_pts_to_cell gC #1.0R
-              mrow mcol
-              (threadRow * tm + ii) threadCol v)) **
-        gpu
+  // Pulse.Lib.Array.pts_to_len rchProd;
+  let mut resIdxM = 0sz;
+  while (SZ.(!resIdxM <^ tm))
+    invariant
+      exists* (vresIdxM : sz{vresIdxM <= tm}) (vrchProd : lseq et (tm*tn)).
+        (resIdxM |-> vresIdxM) **
+        (rchProd |-> vrchProd)
   {
-    let vresIdx = !resIdx;
-    forevery_extract #(natlt tm) (SZ.v vresIdx) _;
+    let mut resIdxN = 0sz;
+    while (SZ.(!resIdxN <^ tn))
+      invariant
+        exists* (vresIdxN : sz{vresIdxN <= tn}) (vrchProd : lseq et (tm*tn)).
+          (resIdxN |-> vresIdxN) **
+          (rchProd |-> vrchProd)
+    {
+      let vresIdxM = !resIdxM;
+      let vresIdxN = !resIdxN;
 
-    let innerTileRow = threadRow *^ tm +^ vresIdx;
-    with bi0 bj0 i0 j0 v0.
-      rewrite m4_pts_to_cell gC bi0  bj0  i0   j0   v0
-          as m4_pts_to_cell gC mrow mcol (threadRow * tm + vresIdx) threadCol v0;
+      (* get separate access to the thread's current cell in gC *)
+      forevery_extract #(natlt tm & natlt tn) (Mktuple2 #(natlt tm) #(natlt tn) (SZ.v vresIdxM) (SZ.v vresIdxN)) _;
 
-    let v0 = M4.gpu_matrix_read_cell gC mrow mcol (threadRow *^ tm +^ vresIdx) threadCol;
-    open Pulse.Lib.Array;
-    let v1 = cache1d.(!resIdx);
-    let v' = comb v0 v1;
-    M4.gpu_matrix_write_cell gC mrow mcol (threadRow *^ tm +^ vresIdx) threadCol v';
+      (* read the current cell in gC *)
+      with bi0 bj0 i0 j0 v0.
+        rewrite m4_pts_to_cell gC bi0  bj0  i0   j0   v0
+            as m4_pts_to_cell gC mrow mcol (threadRow * tm + vresIdxM) (threadCol *^ tn +^ vresIdxN) v0;
+      let v0 = M4.gpu_matrix_read_cell gC mrow mcol (threadRow *^ tm +^ vresIdxM) (threadCol *^ tn +^ vresIdxN);
 
-    with bi0 bj0 i0 j0 v0.
-      rewrite m4_pts_to_cell gC bi0  bj0  i0   j0   v0
-          as m4_pts_to_cell gC mrow mcol (threadRow * tm + vresIdx) threadCol v0;
+      (* add the new result in the register cache to the value from gC and overwrite the the cell in gC *)
+      open Pulse.Lib.Array;
+      let v1 = rchProd.(!resIdxM *^ tn +^ !resIdxN);
+      let v' = comb v0 v1;
+      M4.gpu_matrix_write_cell gC mrow mcol (threadRow *^ tm +^ vresIdxM) (threadCol *^ tn +^ vresIdxN) v';
+      with bi0 bj0 i0 j0 v0.
+        rewrite m4_pts_to_cell gC bi0  bj0  i0   j0   v0
+            as m4_pts_to_cell gC mrow mcol (threadRow * tm + vresIdxM) (threadCol *^ tn +^ vresIdxN) v0;
 
-    resIdx := !resIdx +^ 1sz;
-    Pulse.Lib.Trade.elim_trade
-      (exists* v.
-        m4_pts_to_cell gC #1.0R
-          mrow mcol
-          (threadRow * tm + vresIdx) threadCol v)
-      (forall+ (ii : natlt tm).
+      (* return separate access to the thread's current cellin gC *)
+      Pulse.Lib.Trade.elim_trade
         (exists* v.
           m4_pts_to_cell gC #1.0R
             mrow mcol
-            (threadRow * tm + ii) threadCol v));
+            (threadRow * tm + vresIdxM) (threadCol * tn + vresIdxN) v)
+        (forall+ (ii : (natlt tm & natlt tn)).
+          (exists* v.
+            m4_pts_to_cell gC #1.0R
+              mrow mcol
+              (threadRow * tm + ii._1) (threadCol * tn + ii._2) v));
+
+      resIdxN := !resIdxN +^ 1sz;
+    };
+
+    resIdxM := !resIdxM +^ 1sz;
   };
 
   M.gpu_matrix_concr sA; rewrite each M.core sA as sarA;
   M.gpu_matrix_concr sB; rewrite each M.core sB as sarB;
 
-  fold barrier_tok tm slA slB sarA sarB (2 * mshared) tid;
+  fold barrier_tok slA slB sarA sarB (2 * mshared) (bm/tm * (bn/tn)) tid;
 
   rewrite each sarA as fst sh;
   rewrite each sarB as fst (snd sh);
 
   ghost
-  fn raux (i: natlt tm)
+  fn raux (i: (natlt tm & natlt tn))
   requires
     (exists* (v: et).
       M4.gpu_matrix_pts_to_cell #et #(SZ.v mrows) #(SZ.v mcols) #(SZ.v bm)
         #(SZ.v bn) #lC gC #1.0R (SZ.v mrow)
-        (SZ.v mcol) (SZ.v threadRow * SZ.v tm + i)
-        (SZ.v threadCol) v)
+        (SZ.v mcol) (SZ.v threadRow * SZ.v tm + i._1)
+        (SZ.v threadCol * SZ.v tn + i._2) v)
   ensures
     (exists* (v: et).
       M4.gpu_matrix_pts_to_cell #et #(SZ.v mrows) #(SZ.v mcols) #(SZ.v bm)
         #(SZ.v bn) #lC gC #1.0R (SZ.v bid / SZ.v mcols)
-        (SZ.v bid % SZ.v mcols) (SZ.v tid / SZ.v bn * SZ.v tm + i)
-        (SZ.v tid % SZ.v bn) v)
+        (SZ.v bid % SZ.v mcols) (SZ.v tid / (SZ.v bn / SZ.v tn) * SZ.v tm + i._1)
+        (SZ.v tid % (SZ.v bn / SZ.v tn) * SZ.v tn + i._2) v)
   {
     with v. _;
-    rewrite each SZ.v mrow as SZ.v (bid /^ mcols),
-                 SZ.v mcol as SZ.v (bid %^ mcols),
-                 SZ.v threadRow as SZ.v (tid /^ bn),
-                 SZ.v threadCol as SZ.v (tid %^ bn);
     rewrite
       (M4.gpu_matrix_pts_to_cell #et #(SZ.v mrows) #(SZ.v mcols) #(SZ.v bm)
-          #(SZ.v bn) #lC gC #1.0R (SZ.v (bid /^ mcols))
-          (SZ.v (bid %^ mcols)) (SZ.v (tid /^ bn) * SZ.v tm + i)
-          (SZ.v (tid %^ bn)) v)
+        #(SZ.v bn) #lC gC #1.0R (SZ.v mrow)
+        (SZ.v mcol) (SZ.v threadRow * SZ.v tm + i._1)
+        (SZ.v threadCol * SZ.v tn + i._2) v)
     as
       (M4.gpu_matrix_pts_to_cell #et #(SZ.v mrows) #(SZ.v mcols) #(SZ.v bm)
-          #(SZ.v bn) #lC gC #1.0R (SZ.v bid / SZ.v mcols)
-          (SZ.v bid % SZ.v mcols) (SZ.v tid / SZ.v bn * SZ.v tm + i)
-          (SZ.v tid % SZ.v bn) v);
+        #(SZ.v bn) #lC gC #1.0R (SZ.v bid / SZ.v mcols)
+        (SZ.v bid % SZ.v mcols) (SZ.v tid / (SZ.v bn / SZ.v tn) * SZ.v tm + i._1)
+        (SZ.v tid % (SZ.v bn / SZ.v tn) * SZ.v tn + i._2) v);
     ()
   };
   forevery_map _ _ raux;
+  forevery_unflatten #(natlt tm) #_ #(natlt tn) (fun i -> fun j ->
+          exists* (v: et).
+            M4.gpu_matrix_pts_to_cell #et #(SZ.v mrows) #(SZ.v mcols) #(SZ.v bm)
+                #(SZ.v bn) #lC gC #1.0R 
+              (SZ.v bid / SZ.v mcols) (SZ.v bid % SZ.v mcols)
+              (SZ.v tid / (SZ.v bn / SZ.v tn) * SZ.v tm + i)
+              (SZ.v tid % (SZ.v bn / SZ.v tn) * SZ.v tn + j)
+              v);
   ()
 }
 #pop-options
@@ -714,13 +764,10 @@ ghost
 fn setup
   (#et : Type0) {| scalar et |}
   (comb : binop et)
-  (#bm #bn #bk : szp)
+  (#bm #bn #bk : szp{SZ.fits (bm * bk) /\ SZ.fits (bk * bn)})
   (#mrows #mshared #mcols : szp)
   (tm : szp{tm /? bm})
-  (#_ : squash (SZ.fits (bm * bk) /\ SZ.fits (bk * bn)))
-  // because of how the original code loads into shmem,
-  //  the following is required
-  (#_: squash ((bm/tm * bn) == bm * bk /\ (bm/tm * bn) == bn * bk))
+  (tn : szp{tn /? bn})
   (#lA : mlayout4 mrows   mshared bm bk)
   (#lB : mlayout4 mshared mcols   bk bn)
   (#lC : mlayout4 mrows   mcols   bm bn)
@@ -740,8 +787,8 @@ fn setup
     (gC |-> eC)
   ensures
     (forall+ (bid : natlt (mrows *^ mcols))
-             (tid : natlt (bm /^ tm *^ bn)).
-      kpre1 comb tm gA gB gC eA eB fA fB bid tid) **
+             (tid : natlt (bm /^ tm *^ (bn /^ tn))).
+      kpre1 comb tm tn gA gB gC eA eB fA fB bid tid) **
     emp (* frame *)
 {
   admit();
@@ -751,11 +798,10 @@ ghost
 fn block_setup
   (#et : Type0) {| scalar et |}
   (comb : binop et)
-  (#bm #bn #bk : szp)
+  (#bm #bn #bk : szp{SZ.fits (bm * bk) /\ SZ.fits (bk * bn)})
   (#mrows #mshared #mcols : szp)
   (tm : szp{tm /? bm})
-  (#_ : squash (SZ.fits (bm * bk) /\ SZ.fits (bk * bn)))
-  (#_: squash ((bm/tm * bn) == bm * bk /\ (bm/tm * bn) == bn * bk))
+  (tn : szp{tn /? bn})
   (slA : mlayout bm bk)
   (slB : mlayout bk bn)
   (#lA : mlayout4 mrows   mshared bm bk)
@@ -774,14 +820,14 @@ fn block_setup
   (bid : natlt (mrows *^ mcols))
   ()
   requires
-    block_setup_tok (bm /^ tm *^ bn) **
+    block_setup_tok (bm /^ tm *^ (bn /^ tn)) **
     live_c_shmems sh **
-    (forall+ (tid : natlt (bm/^tm *^ bn)).
-      kpre1 comb tm gA gB gC eA eB fA fB bid tid)
+    (forall+ (tid : natlt (bm/^tm *^ (bn /^ tn))).
+      kpre1 comb tm tn gA gB gC eA eB fA fB bid tid)
   ensures
-    block_setup_tok (bm/^tm *^ bn) **
-    (forall+ (tid : natlt (bm/^tm *^ bn)).
-      kpre comb tm slA slB gA gB gC eA eB fA fB sh bid tid) **
+    block_setup_tok (bm/^tm *^ (bn /^ tn)) **
+    (forall+ (tid : natlt (bm/^tm *^ (bn /^ tn))).
+      kpre comb tm tn slA slB gA gB gC eA eB fA fB sh bid tid) **
     emp (* frame *)
 {
   admit();
@@ -791,11 +837,10 @@ ghost
 fn block_teardown
   (#et : Type0) {| scalar et |}
   (comb : binop et)
-  (#bm #bn #bk : szp)
+  (#bm #bn #bk : szp{SZ.fits (bm * bk) /\ SZ.fits (bk * bn)})
   (#mrows #mshared #mcols : szp)
   (tm : szp{tm /? bm})
-  (#_ : squash (SZ.fits (bm * bk) /\ SZ.fits (bk * bn)))
-  (#_: squash ((bm/tm * bn) == bm * bk /\ (bm/tm * bn) == bn * bk))
+  (tn : szp{tn /? bn})
   (slA : mlayout bm bk)
   (slB : mlayout bk bn)
   (#lA : mlayout4 mrows   mshared bm bk)
@@ -814,13 +859,13 @@ fn block_teardown
   (bid : natlt (mrows *^ mcols))
   ()
   requires
-    (forall+ (tid : natlt (bm/^tm *^ bn)).
-      kpost comb tm slA slB gA gB gC eA eB fA fB sh bid tid) **
+    (forall+ (tid : natlt (bm/^tm *^ (bn /^ tn))).
+      kpost comb tm tn slA slB gA gB gC eA eB fA fB sh bid tid) **
     emp (* frame *)
   ensures
     live_c_shmems sh **
-    (forall+ (tid : natlt (bm/^tm *^ bn)).
-      kpost1 comb tm gA gB gC eA eB fA fB bid tid)
+    (forall+ (tid : natlt (bm/^tm *^ (bn /^ tn))).
+      kpost1 comb tm tn gA gB gC eA eB fA fB bid tid)
 {
   admit();
 }
@@ -829,11 +874,10 @@ ghost
 fn teardown
   (#et : Type0) {| scalar et |}
   (comb : binop et)
-  (#bm #bn #bk : szp)
+  (#bm #bn #bk : szp{SZ.fits (bm * bk) /\ SZ.fits (bk * bn)})
   (#mrows #mshared #mcols : szp)
   (tm : szp{tm /? bm})
-  (#_ : squash (SZ.fits (bm * bk) /\ SZ.fits (bk * bn)))
-  (#_: squash ((bm/tm * bn) == bm * bk /\ (bm/tm * bn) == bn * bk))
+  (tn : szp{tn /? bn})
   (#lA : mlayout4 mrows   mshared bm bk)
   (#lB : mlayout4 mshared mcols   bk bn)
   (#lC : mlayout4 mrows   mcols   bm bn)
@@ -849,8 +893,8 @@ fn teardown
   ()
   requires
     (forall+ (bid : natlt (mrows *^ mcols))
-             (tid : natlt (bm /^ tm *^ bn)).
-      kpost1 comb tm gA gB gC eA eB fA fB bid tid) **
+             (tid : natlt (bm /^ tm *^ (bn /^ tn))).
+      kpost1 comb tm tn gA gB gC eA eB fA fB bid tid) **
     emp (* frame *)
   ensures
     (gA |-> Frac fA eA) **
@@ -874,8 +918,7 @@ let mk_kernel
   (#bm #bn #bk : szp)
   (#mrows #mshared #mcols : szp)
   (tm : szp{tm /? bm})
-  (#_: squash ((bm/tm * bn) == bm * bk /\ (bm/tm * bn) == bn * bk))
-  (#_ : squash (SZ.fits (bm * bk) /\ SZ.fits (bk * bn)))
+  (tn : szp{tn /? bn})
   (slA : mlayout bm bk)
   (slB : mlayout bk bn)
   {| clayout slA, clayout slB |}
@@ -892,30 +935,30 @@ let mk_kernel
   (#eB : ematrix4 et mshared mcols bk bn)
   (#eC : ematrix4 et mrows mcols bm bn)
   (_ : squash (mrows * mcols <= max_blocks
-               /\ (bm/tm * bn) <= max_threads))
+               /\ (bm/tm * (bn/tn)) <= max_threads))
   : kernel_desc
       ((gA |-> Frac fA eA) ** (gB |-> Frac fB eB) ** (gC |-> eC))
       ((gA |-> Frac fA eA) ** (gB |-> Frac fB eB) ** (gC |-> MS.mmcomb comb eC eA eB))
 = {
-  nblk = mrows *^ mcols; //SZ.uint_to_t (SZ.v mrows * SZ.v mcols);
-  nthr = (bm /^ tm *^ bn);
+  nblk = mrows *^ mcols;
+  nthr = (bm /^ tm *^ (bn /^ tn));
 
   shmems_desc = shmems_desc et bm bn bk;
 
   frame = emp;
-  block_pre  = (fun bid -> forall+ (tid : natlt (bm/^tm *^ bn)). kpre1  comb tm gA gB gC eA eB fA fB bid tid);
-  block_post = (fun bid -> forall+ (tid : natlt (bm/^tm *^ bn)). kpost1 comb tm gA gB gC eA eB fA fB bid tid);
-  setup      = setup    comb tm gA gB gC #eA #eB #eC;
-  teardown   = teardown comb tm gA gB gC #eA #eB #eC;
+  block_pre  = (fun bid -> forall+ (tid : natlt (bm/^tm *^ (bn/^tn))). kpre1  comb tm tn gA gB gC eA eB fA fB bid tid);
+  block_post = (fun bid -> forall+ (tid : natlt (bm/^tm *^ (bn/^tn))). kpost1 comb tm tn gA gB gC eA eB fA fB bid tid);
+  setup      = setup    comb tm tn gA gB gC #eA #eB #eC;
+  teardown   = teardown comb tm tn gA gB gC #eA #eB #eC;
 
   block_frame    = (fun _ar _bid -> emp);
-  block_setup    =  block_setup    comb tm slA slB gA gB gC #eA #eB #eC;
-  block_teardown = block_teardown comb tm slA slB gA gB gC #eA #eB #eC;
+  block_setup    = block_setup comb tm tn slA slB gA gB gC #eA #eB #eC;
+  block_teardown = block_teardown comb tm tn slA slB gA gB gC #eA #eB #eC;
 
-  kpre      = kpre  comb tm slA slB gA gB gC eA eB fA fB;
-  kpost     = kpost comb tm slA slB gA gB gC eA eB fA fB;
+  kpre      = kpre  comb tm tn slA slB gA gB gC eA eB fA fB;
+  kpost     = kpost comb tm tn slA slB gA gB gC eA eB fA fB;
 
-  f = kf comb tm slA slB gA #fA gB #fB gC #eA #eB;
+  f = kf comb tm tn slA slB gA #fA gB #fB gC #eA #eB;
 }
 
 inline_for_extraction noextract
@@ -925,7 +968,9 @@ fn mmcomb_gpu
   (#bm #bn #bk : szp)
   (#mrows #mshared #mcols : szp)
   (tm : szp{tm /? bm})
-  (#_: squash ((bm/tm * bn) == bm * bk /\ (bm/tm * bn) == bn * bk))
+  (tn : szp{tn /? bn})
+  (slA : mlayout bm bk)
+  (slB : mlayout bk bn)
   (#lA : mlayout4 mrows   mshared bm bk)
   (#lB : mlayout4 mshared mcols   bk bn)
   (#lC : mlayout4 mrows   mcols   bm bn)
@@ -944,11 +989,11 @@ fn mmcomb_gpu
     (gB |-> Frac fB eB)
   requires
     pure (mrows * mcols <= max_blocks) **
-    pure (bm/tm * bn <= max_threads) **
+    pure (bm/tm * (bn/tn) <= max_threads) **
     (gC |-> eC)
   ensures
     gC |-> MS.mmcomb comb eC eA eB
 {
   (* fixed the inner layouts, or we'd have to propagate this everywhere? *)
-  launch_sync (mk_kernel comb tm (R.row_major _ _) (R.row_major _ _) gA gB gC ());
+  launch_sync (mk_kernel comb tm tn (R.row_major _ _) (R.row_major _ _) gA gB gC ());
 }
